theories/iris/language/iris_ewp_ctx.v
@@ -36,40 +36,40 @@ Definition ewp_wasm_ctx_frame `{!wasmG Σ}
 (* Context wps for blocks *)
  Notation "'EWP' e 'UNDER' f @ E 'CTX' i ; lh <| Ψ |> {{ Φ } }" := (ewp_wasm_ctx E e%E f Ψ Φ i lh)
   (at level 20, e, Ψ, Φ, lh at level 200, only parsing) : bi_scope. 
-Notation "'EWP' e 'UNDER' f @ E 'CTX' i ; lh {{ Φ } }" := (ewp_wasm_ctx E e%E f ( λ _, iProt_bottom ) Φ i lh)
+Notation "'EWP' e 'UNDER' f @ E 'CTX' i ; lh {{ Φ } }" := (ewp_wasm_ctx E e%E f meta_bottom Φ i lh)
   (at level 20, e, Φ, lh at level 200, only parsing) : bi_scope.
  Notation "'EWP' e 'UNDER' f 'CTX' i ; lh <| Ψ |> {{ Φ } }" := (ewp_wasm_ctx ⊤ e%E f Ψ Φ i lh)
   (at level 20, e, Ψ, Φ, lh at level 200, only parsing) : bi_scope. 
-Notation "'EWP' e 'UNDER' f 'CTX' i ; lh {{ Φ } }" := (ewp_wasm_ctx ⊤ e%E f ( λ _, iProt_bottom ) Φ i lh)
+Notation "'EWP' e 'UNDER' f 'CTX' i ; lh {{ Φ } }" := (ewp_wasm_ctx ⊤ e%E f meta_bottom Φ i lh)
                                               (at level 20, e, Φ, lh at level 200, only parsing) : bi_scope.
 
 (* Empty context *)
  Notation "'EWP' e 'UNDER' f @ E 'CTX_EMPTY' <| Ψ |> {{ Φ } }" := (ewp_wasm_ctx E e%E f Ψ Φ 0 (LH_base [] []))
                                                          (at level 20, e, Ψ, Φ at level 200, only parsing) : bi_scope. 
-Notation "'EWP' e 'UNDER' f @ E 'CTX_EMPTY' {{ Φ } }" := (ewp_wasm_ctx E e%E f (λ _, iProt_bottom) Φ 0 (LH_base [] []))
+Notation "'EWP' e 'UNDER' f @ E 'CTX_EMPTY' {{ Φ } }" := (ewp_wasm_ctx E e%E f meta_bottom Φ 0 (LH_base [] []))
                                                  (at level 20, e, Φ at level 200, only parsing) : bi_scope.
  Notation "'EWP' e 'UNDER' f 'CTX_EMPTY' <| Ψ |> {{ Φ } }" := (ewp_wasm_ctx ⊤ e%E f Ψ Φ 0 (LH_base [] []))
                                                      (at level 20, e, Ψ, Φ at level 200, only parsing) : bi_scope. 
-Notation "'EWP' e 'UNDER' f 'CTX_EMPTY' {{ Φ } }" := (ewp_wasm_ctx ⊤ e%E f (λ _, iProt_bottom) Φ 0 (LH_base [] []))
+Notation "'EWP' e 'UNDER' f 'CTX_EMPTY' {{ Φ } }" := (ewp_wasm_ctx ⊤ e%E f meta_bottom Φ 0 (LH_base [] []))
                                                  (at level 20, e, Φ at level 200, only parsing) : bi_scope.
 
 (* With explicit v *)
 
  Notation "'EWP' e 'UNDER' f @ E 'CTX' i ; lh <| Ψ |> {{ v ; h , Φ } }" := (ewp_wasm_ctx E e%E f Ψ (λ v h, Φ) i lh)
   (at level 20, e, v, Ψ, Φ, lh at level 200, only parsing) : bi_scope. 
-Notation "'EWP' e 'UNDER' f @ E 'CTX' i ; lh {{ v ; h , Φ } }" := (ewp_wasm_ctx E e%E f (λ _, iProt_bottom) (λ v h, Φ) i lh)
+Notation "'EWP' e 'UNDER' f @ E 'CTX' i ; lh {{ v ; h , Φ } }" := (ewp_wasm_ctx E e%E f meta_bottom (λ v h, Φ) i lh)
   (at level 20, e, v, Φ, lh at level 200, only parsing) : bi_scope.
  Notation "'EWP' e 'UNDER' f 'CTX' i ; lh <| Ψ |> {{ v ; h , Φ } }" := (ewp_wasm_ctx ⊤ e%E f Ψ (λ v h, Φ) i lh)
   (at level 20, e, v, Ψ, Φ, lh at level 200, only parsing) : bi_scope. 
-Notation "'EWP' e 'UNDER' f 'CTX' i ; lh {{ v ; h , Φ } }" := (ewp_wasm_ctx ⊤ e%E f (λ _, iProt_bottom) (λ v h, Φ) i lh)
+Notation "'EWP' e 'UNDER' f 'CTX' i ; lh {{ v ; h , Φ } }" := (ewp_wasm_ctx ⊤ e%E f meta_bottom (λ v h, Φ) i lh)
                                               (at level 20, e, v, Φ, lh at level 200, only parsing) : bi_scope.
  Notation "'EWP' e 'UNDER' f @ E 'CTX_EMPTY' <| Ψ |> {{ v ; h , Φ } }" := (ewp_wasm_ctx E e%E f Ψ (λ v h, Φ) 0 (LH_base [] []))
                                                          (at level 20, e, v, Ψ, Φ at level 200, only parsing) : bi_scope. 
-Notation "'EWP' e 'UNDER' f @ E 'CTX_EMPTY' {{ v ; h , Φ } }" := (ewp_wasm_ctx E e%E f (λ _, iProt_bottom) (λ v, Φ) 0 (LH_base [] []))
+Notation "'EWP' e 'UNDER' f @ E 'CTX_EMPTY' {{ v ; h , Φ } }" := (ewp_wasm_ctx E e%E f meta_bottom (λ v, Φ) 0 (LH_base [] []))
                                                  (at level 20, e, v, Φ at level 200, only parsing) : bi_scope.
  Notation "'EWP' e 'UNDER' f 'CTX_EMPTY' <| Ψ |> {{ v ; h , Φ } }" := (ewp_wasm_ctx ⊤ e%E f Ψ (λ v h, Φ) 0 (LH_base [] []))
                                                      (at level 20, e, v, Ψ, Φ at level 200, only parsing) : bi_scope. 
-Notation "'EWP' e 'UNDER' f 'CTX_EMPTY' {{ v ; h , Φ } }" := (ewp_wasm_ctx ⊤ e%E f (λ _, iProt_bottom) (λ v h, Φ) 0 (LH_base [] []))
+Notation "'EWP' e 'UNDER' f 'CTX_EMPTY' {{ v ; h , Φ } }" := (ewp_wasm_ctx ⊤ e%E f meta_bottom (λ v h, Φ) 0 (LH_base [] []))
                                                  (at level 20, e, v, Φ at level 200, only parsing) : bi_scope.
 
 
@@ -90,17 +90,17 @@ Notation "'EWP' e 'UNDER' f 'CTX_EMPTY' {{ v ; h , Φ } }" := (ewp_wasm_ctx ⊤ 
     format "'[hv' 'EWP'  e  '/' 'UNDER'  g  @  '[' '/' E  ']' 'FRAME'  '/' '[' n ;  '/' f ']'  '/' 'CTX_EMPTY'  '/' <| '[' Ψ ']' |> '/' {{  '[' v ; h ,  '/' Q  ']' } } ']'") : bi_scope. 
 
 (* no Ψ *)
-Notation "'EWP' e 'UNDER' g @ E 'FRAME' n ; f {{ Φ } }" := (ewp_wasm_frame E e%E g (λ _, iProt_bottom) Φ n f)
+Notation "'EWP' e 'UNDER' g @ E 'FRAME' n ; f {{ Φ } }" := (ewp_wasm_frame E e%E g meta_bottom Φ n f)
   (at level 20, e, Φ, n, f at level 200, only parsing) : bi_scope.
 
-Notation "'EWP' e 'UNDER' g @ E 'FRAME' n ; f {{ v ; h , Q } }" := (ewp_wasm_frame E e%E g (λ _, iProt_bottom) (λ v h, Q) n f)
+Notation "'EWP' e 'UNDER' g @ E 'FRAME' n ; f {{ v ; h , Q } }" := (ewp_wasm_frame E e%E g meta_bottom (λ v h, Q) n f)
   (at level 20, e, v, Q, n, f at level 200,
     format "'[hv' 'EWP'  e  '/' 'UNDER'  g  @  '[' '/' E  ']' 'FRAME'  '/' '[' n ;  '/' f ']'  '/' {{  '[' v ; h ,  '/' Q  ']'  } } ']'") : bi_scope.
 
-Notation "'EWP' e 'UNDER' g @ E 'FRAME' n ; f 'CTX' i ; lh {{ v ; h , Q } }" := (ewp_wasm_ctx_frame E e%E g (λ _, iProt_bottom) (λ v h, Q) n f i lh)
+Notation "'EWP' e 'UNDER' g @ E 'FRAME' n ; f 'CTX' i ; lh {{ v ; h , Q } }" := (ewp_wasm_ctx_frame E e%E g meta_bottom (λ v h, Q) n f i lh)
   (at level 20, e, n, f, Q, lh at level 200,
    format "'[hv' 'EWP'  e  '/' 'UNDER'  g  @  '[' '/' E  ']' 'FRAME'  '/' '[' n ;  '/' f ']'  '/' 'CTX'  '/' '[' i ;  '/' lh ']'  '/' {{  '[' v ; h ,  '/' Q  ']'   } } ']'") : bi_scope.
-Notation "'EWP' e 'UNDER' g @ E 'FRAME' n ; f 'CTX_EMPTY' {{ v ; h , Q } }" := (ewp_wasm_ctx_frame E e%E g (λ _, iProt_bottom) (λ v h, Q) n f 0 (LH_base [] []))
+Notation "'EWP' e 'UNDER' g @ E 'FRAME' n ; f 'CTX_EMPTY' {{ v ; h , Q } }" := (ewp_wasm_ctx_frame E e%E g meta_bottom (λ v h, Q) n f 0 (LH_base [] []))
   (at level 20, e, n, f, Q at level 200,
     format "'[hv' 'EWP'  e  '/' 'UNDER'  g  @  '[' '/' E  ']' 'FRAME'  '/' '[' n ;  '/' f ']'  '/' 'CTX_EMPTY'  '/' {{  '[' v ; h ,  '/' Q  ']'  } } ']'") : bi_scope.
 
@@ -120,17 +120,17 @@ Notation "'EWP' e 'UNDER' g 'FRAME' n ; f 'CTX_EMPTY' <| Ψ |> {{ v ; h , Q } }"
     format "'[hv' 'EWP'  e  '/' 'UNDER'  g  'FRAME'  '/' '[' n ;  '/' f ']'  '/' 'CTX_EMPTY'  '/' <| '[' Ψ ']' |> '/' {{  '[' v ; h ,  '/' Q  ']'  } } ']'") : bi_scope. 
 
 (* no Ψ, no @E *)
-Notation "'EWP' e 'UNDER' g 'FRAME' n ; f {{ Φ } }" := (ewp_wasm_frame ⊤ e%E g (λ _, iProt_bottom) Φ n f)
+Notation "'EWP' e 'UNDER' g 'FRAME' n ; f {{ Φ } }" := (ewp_wasm_frame ⊤ e%E g meta_bottom Φ n f)
   (at level 20, e, f, Φ, n at level 200, only parsing) : bi_scope.
 
-Notation "'EWP' e 'UNDER' g 'FRAME' n ; f {{ v ; h , Q } }" := (ewp_wasm_frame ⊤ e%E g (λ _, iProt_bottom) (λ v h, Q) n f)
+Notation "'EWP' e 'UNDER' g 'FRAME' n ; f {{ v ; h , Q } }" := (ewp_wasm_frame ⊤ e%E g meta_bottom (λ v h, Q) n f)
   (at level 20, e, v, Q, n, f at level 200,
     format "'[hv' 'EWP'  e  '/' 'UNDER'  g  'FRAME'  '/' '[' n ;  '/' f ']'  '/' {{  '[' v ; h ,  '/' Q  ']'  } } ']'") : bi_scope.
 
-Notation "'EWP' e 'UNDER' g 'FRAME' n ; f 'CTX' i ; lh {{ v ; h , Q } }" := (ewp_wasm_ctx_frame ⊤ e%E g (λ _, iProt_bottom) (λ v h, Q) n f i lh)
+Notation "'EWP' e 'UNDER' g 'FRAME' n ; f 'CTX' i ; lh {{ v ; h , Q } }" := (ewp_wasm_ctx_frame ⊤ e%E g meta_bottom (λ v h, Q) n f i lh)
   (at level 20, e, n, f, Q, lh at level 200,
    format "'[hv' 'EWP'  e  '/' 'UNDER'  g  'FRAME'  '/' '[' n ;  '/' f ']'  '/' 'CTX'  '/' '[' i ;  '/' lh ']'  '/' {{  '[' v ; h ,  '/' Q  ']'   } } ']'") : bi_scope.
-Notation "'EWP' e 'UNDER' g 'FRAME' n ; f 'CTX_EMPTY' {{ v ; h , Q } }" := (ewp_wasm_ctx_frame ⊤ e%E g (λ _, iProt_bottom) (λ v h, Q) n f 0 (LH_base [] []))
+Notation "'EWP' e 'UNDER' g 'FRAME' n ; f 'CTX_EMPTY' {{ v ; h , Q } }" := (ewp_wasm_ctx_frame ⊤ e%E g meta_bottom (λ v h, Q) n f 0 (LH_base [] []))
   (at level 20, e, n, f, Q at level 200,
    format "'[hv' 'EWP'  e  '/' 'UNDER'  g  'FRAME'  '/' '[' n ;  '/' f ']'  '/' 'CTX_EMPTY'  '/' {{  '[' v ; h ,  '/' Q  ']'  } } ']'") : bi_scope.
 
